Ajout de fermeture de terme + pistes à explorer

.CoqMakefile.d
@@ -1,33 +1,33 @@
-src/Canonical_form.vo src/Canonical_form.glob src/Canonical_form.v.beautified src/Canonical_form.required_vo: src/Canonical_form.v src/Syntax.vo src/Types.vo src/Hints.vo
-src/Canonical_form.vio: src/Canonical_form.v src/Syntax.vio src/Types.vio src/Hints.vio
-src/Canonical_form.vos src/Canonical_form.vok src/Canonical_form.required_vos: src/Canonical_form.v src/Syntax.vos src/Types.vos src/Hints.vos
-src/Free.vo src/Free.glob src/Free.v.beautified src/Free.required_vo: src/Free.v src/Maps.vo src/Syntax.vo src/Subst.vo src/Step.vo src/Types.vo src/Hints.vo
-src/Free.vio: src/Free.v src/Maps.vio src/Syntax.vio src/Subst.vio src/Step.vio src/Types.vio src/Hints.vio
-src/Free.vos src/Free.vok src/Free.required_vos: src/Free.v src/Maps.vos src/Syntax.vos src/Subst.vos src/Step.vos src/Types.vos src/Hints.vos
+src/Canonical_form.vo src/Canonical_form.glob src/Canonical_form.v.beautified src/Canonical_form.required_vo: src/Canonical_form.v src/Hints.vo src/Syntax.vo src/Types.vo src/Maps.vo
+src/Canonical_form.vio: src/Canonical_form.v src/Hints.vio src/Syntax.vio src/Types.vio src/Maps.vio
+src/Canonical_form.vos src/Canonical_form.vok src/Canonical_form.required_vos: src/Canonical_form.v src/Hints.vos src/Syntax.vos src/Types.vos src/Maps.vos
+src/Closed.vo src/Closed.glob src/Closed.v.beautified src/Closed.required_vo: src/Closed.v src/Hints.vo src/Syntax.vo src/Types.vo src/Maps.vo
+src/Closed.vio: src/Closed.v src/Hints.vio src/Syntax.vio src/Types.vio src/Maps.vio
+src/Closed.vos src/Closed.vok src/Closed.required_vos: src/Closed.v src/Hints.vos src/Syntax.vos src/Types.vos src/Maps.vos
 src/Hints.vo src/Hints.glob src/Hints.v.beautified src/Hints.required_vo: src/Hints.v 
 src/Hints.vio: src/Hints.v 
 src/Hints.vos src/Hints.vok src/Hints.required_vos: src/Hints.v 
-src/Main.vo src/Main.glob src/Main.v.beautified src/Main.required_vo: src/Main.v src/Maps.vo src/Syntax.vo src/Subst.vo src/Step.vo src/Types.vo src/Free.vo src/Progress.vo src/Hints.vo
-src/Main.vio: src/Main.v src/Maps.vio src/Syntax.vio src/Subst.vio src/Step.vio src/Types.vio src/Free.vio src/Progress.vio src/Hints.vio
-src/Main.vos src/Main.vok src/Main.required_vos: src/Main.v src/Maps.vos src/Syntax.vos src/Subst.vos src/Step.vos src/Types.vos src/Free.vos src/Progress.vos src/Hints.vos
 src/Maps.vo src/Maps.glob src/Maps.v.beautified src/Maps.required_vo: src/Maps.v 
 src/Maps.vio: src/Maps.v 
 src/Maps.vos src/Maps.vok src/Maps.required_vos: src/Maps.v 
-src/Maps_func.vo src/Maps_func.glob src/Maps_func.v.beautified src/Maps_func.required_vo: src/Maps_func.v 
-src/Maps_func.vio: src/Maps_func.v 
-src/Maps_func.vos src/Maps_func.vok src/Maps_func.required_vos: src/Maps_func.v 
-src/Progress.vo src/Progress.glob src/Progress.v.beautified src/Progress.required_vo: src/Progress.v src/Maps.vo src/Syntax.vo src/Subst.vo src/Step.vo src/Types.vo src/Free.vo src/Canonical_form.vo src/Hints.vo
-src/Progress.vio: src/Progress.v src/Maps.vio src/Syntax.vio src/Subst.vio src/Step.vio src/Types.vio src/Free.vio src/Canonical_form.vio src/Hints.vio
-src/Progress.vos src/Progress.vok src/Progress.required_vos: src/Progress.v src/Maps.vos src/Syntax.vos src/Subst.vos src/Step.vos src/Types.vos src/Free.vos src/Canonical_form.vos src/Hints.vos
-src/Step.vo src/Step.glob src/Step.v.beautified src/Step.required_vo: src/Step.v src/Syntax.vo src/Subst.vo src/Hints.vo
-src/Step.vio: src/Step.v src/Syntax.vio src/Subst.vio src/Hints.vio
-src/Step.vos src/Step.vok src/Step.required_vos: src/Step.v src/Syntax.vos src/Subst.vos src/Hints.vos
-src/Subst.vo src/Subst.glob src/Subst.v.beautified src/Subst.required_vo: src/Subst.v src/Syntax.vo src/Hints.vo
-src/Subst.vio: src/Subst.v src/Syntax.vio src/Hints.vio
-src/Subst.vos src/Subst.vok src/Subst.required_vos: src/Subst.v src/Syntax.vos src/Hints.vos
+src/MapsNotations.vo src/MapsNotations.glob src/MapsNotations.v.beautified src/MapsNotations.required_vo: src/MapsNotations.v src/Maps.vo
+src/MapsNotations.vio: src/MapsNotations.v src/Maps.vio
+src/MapsNotations.vos src/MapsNotations.vok src/MapsNotations.required_vos: src/MapsNotations.v src/Maps.vos
+src/Preservation.vo src/Preservation.glob src/Preservation.v.beautified src/Preservation.required_vo: src/Preservation.v src/Hints.vo src/Syntax.vo src/Types.vo src/Subst.vo src/Step.vo src/Canonical_form.vo src/Maps.vo
+src/Preservation.vio: src/Preservation.v src/Hints.vio src/Syntax.vio src/Types.vio src/Subst.vio src/Step.vio src/Canonical_form.vio src/Maps.vio
+src/Preservation.vos src/Preservation.vok src/Preservation.required_vos: src/Preservation.v src/Hints.vos src/Syntax.vos src/Types.vos src/Subst.vos src/Step.vos src/Canonical_form.vos src/Maps.vos
+src/Progress.vo src/Progress.glob src/Progress.v.beautified src/Progress.required_vo: src/Progress.v src/Hints.vo src/Syntax.vo src/Types.vo src/Subst.vo src/Step.vo src/Canonical_form.vo src/Maps.vo
+src/Progress.vio: src/Progress.v src/Hints.vio src/Syntax.vio src/Types.vio src/Subst.vio src/Step.vio src/Canonical_form.vio src/Maps.vio
+src/Progress.vos src/Progress.vok src/Progress.required_vos: src/Progress.v src/Hints.vos src/Syntax.vos src/Types.vos src/Subst.vos src/Step.vos src/Canonical_form.vos src/Maps.vos
+src/Step.vo src/Step.glob src/Step.v.beautified src/Step.required_vo: src/Step.v src/Hints.vo src/Syntax.vo src/Types.vo src/Subst.vo src/Maps.vo
+src/Step.vio: src/Step.v src/Hints.vio src/Syntax.vio src/Types.vio src/Subst.vio src/Maps.vio
+src/Step.vos src/Step.vok src/Step.required_vos: src/Step.v src/Hints.vos src/Syntax.vos src/Types.vos src/Subst.vos src/Maps.vos
+src/Subst.vo src/Subst.glob src/Subst.v.beautified src/Subst.required_vo: src/Subst.v src/Closed.vo src/Hints.vo src/Maps.vo src/Syntax.vo src/Types.vo
+src/Subst.vio: src/Subst.v src/Closed.vio src/Hints.vio src/Maps.vio src/Syntax.vio src/Types.vio
+src/Subst.vos src/Subst.vok src/Subst.required_vos: src/Subst.v src/Closed.vos src/Hints.vos src/Maps.vos src/Syntax.vos src/Types.vos
 src/Syntax.vo src/Syntax.glob src/Syntax.v.beautified src/Syntax.required_vo: src/Syntax.v src/Hints.vo
 src/Syntax.vio: src/Syntax.v src/Hints.vio
 src/Syntax.vos src/Syntax.vok src/Syntax.required_vos: src/Syntax.v src/Hints.vos
-src/Types.vo src/Types.glob src/Types.v.beautified src/Types.required_vo: src/Types.v src/Maps.vo src/Syntax.vo src/Step.vo src/Hints.vo
-src/Types.vio: src/Types.v src/Maps.vio src/Syntax.vio src/Step.vio src/Hints.vio
-src/Types.vos src/Types.vok src/Types.required_vos: src/Types.v src/Maps.vos src/Syntax.vos src/Step.vos src/Hints.vos
+src/Types.vo src/Types.glob src/Types.v.beautified src/Types.required_vo: src/Types.v src/Hints.vo src/Maps.vo src/Syntax.vo
+src/Types.vio: src/Types.v src/Hints.vio src/Maps.vio src/Syntax.vio
+src/Types.vos src/Types.vok src/Types.required_vos: src/Types.v src/Hints.vos src/Maps.vos src/Syntax.vos
