src/Step.v
@@ -2,58 +2,96 @@ From Coq Require Import Unicode.Utf8.
 From Coq Require Import Strings.String.
 Local Open Scope Z_scope.
 Require Import ZArith.
-Require Import Syntax.
-Require Import Subst.
 Require Import Hints.
+Require Import Syntax.
+Require Import Types.
+Require Import Subst.
+Require Maps.
+Import Maps.Notations.
 
 Inductive step : expr -> expr -> Prop := 
     | ST_App_Fun : 
-        forall (x : string) (t : type) (e e' v : expr),
+        ∀ (x : string) (t : type) (e e' v : expr),
         value v -> 
         substitution v x e e' ->
         step (E_App (E_Fun x t e) v) e'
     | ST_App_Left : 
-        forall (e1 e1' e2 : expr),
+        ∀ (e1 e1' e2 : expr),
         step e1 e1' ->
         step (E_App e1 e2) (E_App e1' e2)
     | ST_App_Right : 
-        forall (v1 e2 e2' : expr),
+        ∀ (v1 e2 e2' : expr),
         value v1 ->
         step e2 e2' ->
         step (E_App v1 e2) (E_App v1 e2')
     | ST_If_True : 
-        forall (e1 e2 : expr),
+        ∀ (e1 e2 : expr),
         step (E_If E_True e1 e2) e1
     | ST_If_False : 
-        forall (e1 e2 : expr),
+        ∀ (e1 e2 : expr),
         step (E_If E_False e1 e2) e2
     | ST_If : 
-        forall (e1 e1' e2 e3 : expr),
+        ∀ (e1 e1' e2 e3 : expr),
         step e1 e1' ->
         step (E_If e1 e2 e3) (E_If e1' e2 e3)
     | ST_Let_Left : 
-        forall (x : string) (e1 e1' e2 : expr),
+        ∀ (x : string) (e1 e1' e2 : expr),
         step e1 e1' ->
         step (E_Let x e1 e2) (E_Let x e1' e2)
     | ST_Let_Right : 
-        forall (x : string) (v1 e2 e2' : expr),
+        ∀ (x : string) (v1 e2 e2' : expr),
         value v1 ->
         substitution v1 x e2 e2' ->
         step (E_Let x v1 e2) e2'
     | ST_Minus_Left :  
-        forall (e1 e1' e2 : expr),
+        ∀ (e1 e1' e2 : expr),
         step e1 e1' ->
         step (E_Minus e1 e2) (E_Minus e1' e2)
     | ST_Minus_Right :  
-        forall (v1 e2 e2' : expr),
+        ∀ (v1 e2 e2' : expr),
         value v1 ->
         step e2 e2' ->
         step (E_Minus v1 e2) (E_Minus v1 e2')
     | ST_Minus_Num : 
-        forall (z1 z2 : Z),
+        ∀ (z1 z2 : Z),
         step 
             (E_Minus (E_Num z1) (E_Num z2))
             (E_Num (z1 - z2))
 .
 
 Hint Constructors step : local_hints.
+
+
+Local Lemma subst_typing : ∀ Γ s x e e' t_e t_s, 
+    has_type (x |-> t_s; Γ) e t_e ->
+    has_type empty s t_s ->
+    substitution s x e e' -> 
+    has_type Γ e' t_e.
+Proof.
+    intros * H_type_e H_type_s H_subst.
+    generalize dependent t_e.
+    generalize dependent t_s.
+    generalize dependent Γ.
+    induction H_subst; intros;
+    try (inversion H_type_e; subst; eauto with local_hints; fail).
+    - inversion H_type_e; subst. 
+      rewrite Maps.update_eq in H1. inversion H1; subst. apply Types.weakening_empty.
+      assumption.
+    - inversion H_type_e; subst. 
+      apply T_Var. rewrite Maps.update_neq in H2; auto.
+    - inversion H_type_e; subst.
+      apply T_Fun.   
+      rewrite Maps.update_shadow in H4. assumption.    
+    - inversion H_type_e; subst.
+      apply T_Fun.
+      rewrite Maps.update_permute in H6; auto.
+      eapply IHH_subst; eauto.
+
+    - inversion H_type_e; subst. eapply T_Let; eauto.
+      rewrite Maps.update_shadow in H5. auto.
+    - inversion H_type_e; subst. eapply T_Let; eauto.
+      rewrite Maps.update_permute in H7; auto.
+      eapply IHH_subst2; eauto.
+Qed.
+
+Hint Resolve subst_typing : local_hints.
