src/Subst.v
@@ -2,51 +2,60 @@ From Coq Require Import Unicode.Utf8.
 From Coq Require Import Strings.String.
 Local Open Scope Z_scope.
 Require Import ZArith.
-Require Import Syntax.
+Require Import Closed.
 Require Import Hints.
+
+Require Maps.
+Import Maps.Notations.
+Require Import Syntax.
+Require Import Types.
 
 Inductive substitution (s : expr) (x : string) : expr -> expr -> Prop :=
     | S_Var_Eq :
         substitution s x (E_Var x) s
     | S_Var_Neq :
-        forall (y : string), x <> y -> substitution s x (E_Var y) (E_Var y)
+        ∀ (y : string), x <> y -> substitution s x (E_Var y) (E_Var y)
     | S_App : 
-        forall (e1 e1' e2 e2' : expr),
+        ∀ (e1 e1' e2 e2' : expr),
         substitution s x e1 e1' ->
         substitution s x e2 e2' ->
         substitution s x (E_App e1 e2) (E_App e1' e2')
     | S_Fun_Eq : 
-        forall (t : type) (e : expr),
+        ∀ (t : type) (e : expr),
         substitution s x (E_Fun x t e) (E_Fun x t e)
     | S_Fun_Neq : 
-        forall (y : string) (t : type) (e e' : expr),
-        x <> y -> substitution s x e e' -> 
+        ∀ (y: string) (t : type) (e e_aux e' : expr),
+        x <> y ->
+        closed s ->
+        substitution s x e e' -> 
         substitution s x (E_Fun y t e) (E_Fun y t e')
     | S_True : 
         substitution s x E_True E_True
     | S_False : 
         substitution s x E_False E_False
     | S_If : 
-        forall (e1 e1' e2 e2' e3 e3' : expr),
+        ∀ (e1 e1' e2 e2' e3 e3' : expr),
         substitution s x e1 e1' ->
         substitution s x e2 e2' ->
         substitution s x e3 e3' ->
         substitution s x (E_If e1 e2 e3) (E_If e1' e2' e3')
     | S_Let_Eq : 
-        forall (e1 e1' e2: expr),
+        ∀ (e1 e1' e2 : expr),
         substitution s x e1 e1' -> 
         substitution s x (E_Let x e1 e2) (E_Let x e1' e2)
     | S_Let_Neq : 
-        forall (y : string) (e1 e1' e2 e2': expr),
+        ∀ (y : string) (e1 e1' e2 e2': expr),
         x <> y ->
+        closed s ->
         substitution s x e1 e1' -> 
         substitution s x e2 e2' -> 
         substitution s x (E_Let y e1 e2) (E_Let y e1' e2')
+   
     | S_Num : 
-        forall (z : Z),
+        ∀ (z : Z),
         substitution s x (E_Num z) (E_Num z)
     | S_Minus :
-        forall (e1 e1' e2 e2': expr),
+        ∀ (e1 e1' e2 e2': expr),
         substitution s x e1 e1' -> 
         substitution s x e2 e2' -> 
         substitution s x (E_Minus e1 e2) (E_Minus e1' e2')
@@ -54,7 +63,8 @@ Inductive substitution (s : expr) (x : string) : expr -> expr -> Prop :=
 
 Hint Constructors substitution : local_hints.
 
-Local Lemma exists_one : ∀ s x e, ∃ e', substitution s x e e'.
+Local Lemma exists_one : ∀ s x e, closed s -> ∃ e', 
+ substitution s x e e'.
 Proof with eauto.
     intros.
     induction e;
