src/Types.v
@@ -1,55 +1,55 @@
 From Coq Require Import Unicode.Utf8.
-From Coq Require Import Strings.String.
-Local Open Scope Z_scope.
-Require Import ZArith.
-Require Import Maps.
-Require Import Syntax.
-Require Import Step.
 Require Import Hints.
+Require Maps.
+Import Maps.Notations.
+Require Import Syntax.
 
 Definition context := @Maps.map type.
 Definition empty := @Maps.empty type.
 
-
 Inductive has_type : context -> expr -> type -> Prop := 
-| T_Var: forall Γ x t, 
-            Γ ? x = Some t -> 
-            has_type Γ (E_Var x) t
+    | T_Var: ∀ Γ x t, 
+                Γ ? x = Some t -> 
+                has_type Γ (E_Var x) t
 
-| T_Fun: forall Γ x t1 e t2,
-            has_type (x |-> t1; Γ) e t2 ->
-            has_type Γ (E_Fun x t1 e) (Type_Fun t1 t2)
-| T_App: forall Γ e1 e2 t1 t2, 
-            has_type Γ e2 t1 -> 
-            has_type Γ e1 (Type_Fun t1 t2) ->
-            has_type Γ (E_App e1 e2) t2
+    | T_Fun: ∀ Γ x t1 e t2,
+                has_type (x |-> t1; Γ) e t2 ->
+                has_type Γ (E_Fun x t1 e) (Type_Fun t1 t2)
+    | T_App: ∀ Γ e1 e2 t1 t2, 
+                has_type Γ e2 t1 -> 
+                has_type Γ e1 (Type_Fun t1 t2) ->
+                has_type Γ (E_App e1 e2) t2
 
-| T_True: forall Γ, 
-            has_type Γ E_True Type_Bool
-| T_False: forall Γ, 
-            has_type Γ E_True Type_Bool
+    | T_True: ∀ Γ, 
+                has_type Γ E_True Type_Bool
+                
+    | T_False: ∀ Γ, 
+                has_type Γ E_False Type_Bool
 
-| T_If: forall Γ e1 e2 e3 t, 
-            has_type Γ e1 Type_Bool -> 
-            has_type Γ e2 t -> 
-            has_type Γ e3 t -> 
-            has_type Γ (E_If e1 e2 e3) t 
-| T_Let : forall Γ x e1 e2 t1 t2, 
-            has_type Γ e1 t1 -> 
-            has_type (x |-> t1; Γ) e2 t2 -> 
-            has_type Γ (E_Let x e1 e2) t2
-| T_Num : forall Γ z, has_type Γ (E_Num z) Type_Num 
-| T_Minus : forall Γ e1 e2, 
-              has_type Γ e1 Type_Num ->
-              has_type Γ e2 Type_Num ->
-              has_type Γ (E_Minus e1 e2) Type_Num 
-.
+    | T_If: ∀ Γ e1 e2 e3 t, 
+                has_type Γ e1 Type_Bool -> 
+                has_type Γ e2 t -> 
+                has_type Γ e3 t -> 
+                has_type Γ (E_If e1 e2 e3) t 
+
+    | T_Let : ∀ Γ x e1 e2 t1 t2, 
+                has_type Γ e1 t1 -> 
+                has_type (x |-> t1; Γ) e2 t2 -> 
+                has_type Γ (E_Let x e1 e2) t2
+
+    | T_Num : ∀ Γ z, has_type Γ (E_Num z) Type_Num 
+
+    | T_Minus : ∀ Γ e1 e2, 
+                has_type Γ e1 Type_Num ->
+                has_type Γ e2 Type_Num ->
+                has_type Γ (E_Minus e1 e2) Type_Num 
+    .
 
 Hint Constructors has_type : local_hints.
 
 
 Local Lemma weakening : ∀ Γ Γ' e t, 
-    includedin Γ Γ' ->
+    Maps.includedin Γ Γ' ->
     has_type Γ e t ->
     has_type Γ' e t.
 Proof.
@@ -67,7 +67,7 @@ Qed.
 Hint Resolve weakening : local_hints.
 
 
-Lemma weakening_empty : ∀ Γ e t, 
+Local Lemma weakening_empty : ∀ Γ e t, 
     has_type empty e t ->
     has_type Γ e t.
 Proof.
