src/Closed.v
@@ -1,0 +1,155 @@
+From Coq Require Import Unicode.Utf8.
+From Coq Require Import Strings.String.
+Local Open Scope Z_scope.
+Require Import ZArith.
+Require Import Hints.
+Require Import Syntax.
+Require Import Types.
+Require Maps.
+Import Maps.Notations.
+
+(* 
+Variable libre:
+x libre dans e si 
+e = Var x
+e = App e1 e2 => x libre dans e1 ou x libre dans e2
+e = λ y : t . e => y <> x et x libre dans e
+e = If e1 e2 e3 => x libre dans e1 ou x libre dans e2 ou x libre dans e3
+e = Let y e1 e2 => x libre dans e1 ou x <> y et x libre dans e2
+e = Minus e1 e2 => x libre dans e1 ou x libre dans e2
+ *)
+
+Inductive is_free_in (x : string) : expr -> Prop :=
+| Free_Var : is_free_in x (E_Var x)
+| Free_App_Left : 
+    ∀ e₁ e₂, 
+    is_free_in x e₁ -> 
+    is_free_in x (E_App e₁ e₂) 
+| Free_App_Right : 
+    ∀ e₁ e₂, 
+    is_free_in x e₂ -> 
+    is_free_in x (E_App e₁ e₂) 
+| Free_Fun : 
+    ∀ y t e, 
+    y <> x -> 
+    is_free_in x e -> 
+    is_free_in x (E_Fun y t e) 
+| Free_If_Cond : 
+    ∀ e₁ e₂ e₃, 
+    is_free_in x e₁ -> 
+    is_free_in x (E_If e₁ e₂ e₃) 
+| Free_If_Left : 
+    ∀ e₁ e₂ e₃, 
+    is_free_in x e₂ -> 
+    is_free_in x (E_If e₁ e₂ e₃) 
+| Free_If_Right : 
+    ∀ e₁ e₂ e₃, 
+    is_free_in x e₃ -> 
+    is_free_in x (E_If e₁ e₂ e₃) 
+| Free_Let_Left : 
+    ∀ y e₁ e₂, 
+    is_free_in x e₁ -> 
+    is_free_in x (E_Let y e₁ e₂) 
+| Free_Let_Right : 
+    ∀ y e₁ e₂, 
+    y <> x -> is_free_in x e₂ -> 
+    is_free_in x (E_Let y e₁ e₂) 
+| Free_Minus_Left : 
+    ∀ e₁ e₂, 
+    is_free_in x e₁ -> 
+    is_free_in x (E_Minus e₁ e₂) 
+| Free_Minus_Right : 
+    ∀ e₁ e₂, 
+    is_free_in x e₂ -> 
+    is_free_in x (E_Minus e₁ e₂) 
+.
+
+Hint Constructors is_free_in : local_hints.
+
+Definition closed e := ∀ x, ~ is_free_in x e.
+
+Lemma free_has_type :
+    ∀ Γ e t x,
+    is_free_in x e ->
+    has_type Γ e t -> 
+    ∃ t_x, Γ ? x = Some t_x.
+Proof.
+  intros * H_free H_type.
+  generalize dependent Γ.
+  generalize dependent t.
+  induction H_free; intros;
+  try (inversion H_type; subst; eauto);
+  erewrite <- Maps.update_neq;
+  eauto.
+Qed. 
+
+
+Theorem typed_empty :
+    ∀ e t,
+    has_type empty e t -> 
+    closed e.
+Proof.
+    intros * H_type x H_contra.
+    generalize dependent t.
+    induction H_contra; intros;
+    try (inversion H_type; subst; eauto; fail).
+    - inversion H_type; subst. inversion H1.
+    - inversion H_type; subst. 
+      eapply free_has_type in H_contra; eauto.
+      inversion H_contra. rewrite Maps.update_neq in H0; eauto. inversion H0.
+    - inversion H_type; subst. 
+      eapply free_has_type in H_contra; eauto.
+      inversion H_contra. 
+      rewrite Maps.update_neq in H0; eauto. inversion H0.
+Qed.
+
+Lemma closed_app : 
+  ∀ e₁ e₂, 
+  closed (E_App e₁ e₂) -> 
+  closed e₁ /\ closed e₂.
+Proof.
+  intros.
+  unfold closed in *.
+  split; 
+    intros x H_contra;
+    apply H with x;
+    eauto with local_hints.
+Qed.
+
+Lemma closed_let : 
+  ∀ x e₁ e₂, 
+  closed (E_Let x e₁ e₂) -> 
+  closed e₁.
+Proof.
+  intros.
+  unfold closed in *.
+  intros x' H_contra.
+  apply H with x'.
+  eauto with local_hints.
+Qed.
+
+Lemma closed_if : 
+  ∀ e₁ e₂ e₃, 
+  closed (E_If e₁ e₂ e₃) -> 
+  closed e₁ /\ closed e₂ /\ closed e₃.
+Proof.
+  intros.
+  unfold closed in *.
+  repeat split; 
+    intros x H_contra;
+    apply H with x;
+    eauto with local_hints.
+Qed.
+
+Lemma closed_minus : 
+  ∀ e₁ e₂, 
+  closed (E_Minus e₁ e₂) -> 
+  closed e₁ /\ closed e₂.
+Proof.
+  intros.
+  unfold closed in *.
+  split; 
+    intros x H_contra;
+    apply H with x;
+    eauto with local_hints.
+Qed.
