src/Preservation.v
@@ -1,0 +1,30 @@
+From Coq Require Import Unicode.Utf8.
+From Coq Require Import Strings.String.
+Local Open Scope Z_scope.
+Require Import ZArith.
+Require Import Hints.
+Require Import Syntax.
+Require Import Types.
+Require Import Subst.
+Require Import Step.
+Require Import Canonical_form.
+Require Maps.
+Import Maps.Notations.
+
+
+Theorem preservation : ∀ e e' t,
+  has_type empty e t  ->
+  step e e'  ->
+  has_type empty e' t.
+Proof.
+  intros * H_type_e. 
+  generalize dependent e'.
+  remember empty as Γ.
+  induction H_type_e;
+  intros e' H_step; 
+  try (
+    inversion H_step; 
+    subst; 
+    eauto with local_hints).
+  - inversion H_type_e2; subst. eauto with local_hints.
+Qed.
