src/Progress.v
@@ -1,18 +1,17 @@
 From Coq Require Import Unicode.Utf8.
 From Coq Require Import Strings.String.
-Require Import Maps.
 Local Open Scope Z_scope.
 Require Import ZArith.
+Require Import Hints.
 Require Import Syntax.
+Require Import Types.
 Require Import Subst.
 Require Import Step.
-Require Import Types.
-Require Import Free.
 Require Import Canonical_form.
-Require Import Hints.
+Require Maps.
+Import Maps.Notations.
 
 
-Print HintDb local_hints.
 
 
 Theorem expr_progress : ∀ e t,
@@ -20,6 +19,7 @@ Theorem expr_progress : ∀ e t,
     value e \/ ∃ e', step e e'.
 Proof with eauto with local_hints.
     intros * H_type.
+    assert (H_closed := Closed.typed_empty _ _ H_type).
     generalize dependent t.
     induction e; intros;
     try (eauto with local_hints; fail);
@@ -27,26 +27,41 @@ Proof with eauto with local_hints.
 
     - inversion H1.
 
-    - destruct (IHe1 (Type_Fun t1 t)) as [H_val_e1 | [e1' H_step_e1] ]...
-      destruct (IHe2 t1) as [H_val_e2 | [e2' H_step_e2] ]...
-      destruct (Canonical_form.t_fun e1 t1 t H4 H_val_e1) as [x [e' H_eq]]; subst.
-      destruct (IHe1 _ H4) as [H_val | H_ex];
-      [ destruct (Subst.exists_one e2 x e') as [e'0 H_sub] 
-      | destruct H_ex as [e'0 H_ex]]...
+    - apply Closed.closed_app in H_closed as 
+        [H_closed_e1 H_closed_e2]. 
+      destruct (IHe1 H_closed_e1 (Type_Fun t1 t)) as 
+        [H_val_e1 | [e1' H_step_e1] ]...
+      destruct (IHe2 H_closed_e2 t1) as 
+        [H_val_e2 | [e2' H_step_e2] ]...
+      destruct (Canonical_form.t_fun e1 t1 t H4 H_val_e1) as 
+        [x [e' H_eq]]; subst.
+      destruct (IHe1 H_closed_e1 _ H4) as 
+        [H_val | H_ex].
+      + destruct (Subst.exists_one e2 x e') as [e'0 H_sub]...
+      + destruct H_ex as [e'0 H_ex]...
 
-    - destruct (IHe1 _ H3) as [H_val_e1 | [e' H_step]]...
+    - apply Closed.closed_if in H_closed as 
+        [H_closed_e1 H_closed_e2]. 
+      destruct (IHe1 H_closed_e1 _ H3) as 
+        [H_val_e1 | [e' H_step]]...
       apply Canonical_form.t_bool in H_val_e1...
-      destruct H_val_e1 as [H_e1_eq | H_e1_eq]; subst...
+      destruct H_val_e1 as
+         [H_e1_eq | H_e1_eq]; 
+      subst...
 
-    - destruct (IHe1 t1) as [H_val_e1 | [e1' H_step_e1] ]...
+    - apply Closed.closed_let in H_closed. 
+      destruct (IHe1 H_closed t1) as [H_val_e1 | [e1' H_step_e1] ]...
       destruct (Subst.exists_one e1 x e2) as [e' H_sub]...
     
-    - apply IHe1 in H2 as He1. apply IHe2 in H4 as He2.
+    - apply Closed.closed_minus in H_closed as 
+        [H_closed_e1 H_closed_e2].
+      apply IHe1 in H2 as He1... apply IHe2 in H4 as He2...
       destruct He1 as [H_v_e1 | [e1' H_step_e1]]...
       destruct He2 as [H_v_e2 | [e2' H_step_e2]]...
       destruct (Canonical_form.t_num e1 H2 H_v_e1) as [z1 H_z1].
       destruct (Canonical_form.t_num e2 H4 H_v_e2) as [z2 H_z2].
       subst...
+      
 Qed.
 
 Hint Resolve expr_progress : local_hints.
